Hoare_Triple.v
@@ -1,17 +1,17 @@
-From Rela Require Import Vcg.
 From Rela Require Import Com.
+From Rela Require Import Inliner.
 From Rela Require Import Aexp.
 From Rela Require Import Bexp.
 From Rela Require Import Sigma.
 From Rela Require Import Loc.
-Import Why3_Set.
+From Rela Require Import Proc.
 
-(*Defintion of a Hoare Triple*)
+(** Defintion of a Hoare Triple **)
 
 Definition hoare_triple (P Q: assertion) (c : com) (ps : Psi.psi) : Prop :=
   forall s s',  P s -> ceval c s ps s' -> Q s'.
 
-(* Some facts about Hoare Triples *)
+(** Facts about Hoare Triples **)
 
 Lemma seq_hoare_triple :
   forall p1 p2 ps (P Q R: assertion),
@@ -31,17 +31,17 @@ Lemma if_hoare_triple :
     hoare_triple P Q (CIf b p1 p2) ps.
 Proof.
   intros p1 p2 b ps P Q HTrue HFalse s s' HP HE.
-  inversion HE;subst. 
+  inversion HE;subst.
   - unfold hoare_triple in HTrue.
     eapply HTrue.
-    + split. 
-      * apply HP. 
+    + split.
+      * apply HP.
       * assumption.
     + apply H6.
   - unfold hoare_triple in HFalse.
     eapply HFalse.
-    + split. 
-      * apply HP. 
+    + split.
+      * apply HP.
       * assumption.
     + apply H6.
 Qed.
@@ -74,7 +74,7 @@ Proof.
   apply H2.
 Qed.
 
-Lemma while_hoare_triple : 
+Lemma while_hoare_triple :
   forall P b c ps,
     hoare_triple (fun s => P s /\ beval s b = true) (P) c ps ->
     hoare_triple (P) (fun s => P s /\ beval s b = false) (CWhile b c P) ps.
@@ -94,269 +94,107 @@ Proof.
   * inversion Horig.
 Qed.
 
-Lemma proc_hoare_triple : 
-  forall P Q f ps,
-    hoare_triple P Q (fst (ps f)) ps ->
-    hoare_triple P Q (CCall f) ps.
-Proof.
-  intros P Q f ps Hhoare st st' HP Heval.
-  unfold hoare_triple in Hhoare.
-  eapply Hhoare.
-  apply HP.
-  inversion Heval;subst.
-  apply H0.
-Qed.
+(** Definition of Precondtion **)
 
-Definition hoare_triple_proc (ps : Psi.psi) : Prop :=
-  forall p , hoare_triple (get_pre (snd (ps p))) (get_post (snd (ps p))) (CCall p) ps.
+Definition precondition : Type := assertion.
 
-Definition hoare_triple_body (ps : Psi.psi) : Prop :=
-  forall p , hoare_triple (get_pre (snd (ps p))) (get_post (snd (ps p))) (fst (ps p)) ps.
+Definition empty_precondition : precondition := (fun _ => True).
 
-(*to be verified*)
-Axiom recursion_hoare_triple :
+(** Defintion of Postcondtion **)
+
+Definition postcondition : Type := assertion.
+
+Definition empty_postcondition :  postcondition := (fun _ => True).
+
+(** Definition of a procedure contract **)
+
+Definition clause : Type := precondition * postcondition.
+
+Definition empty_clause : clause := (empty_precondition, empty_postcondition).
+
+Definition get_pre (an:clause) :=
+          let (pre,post) := an in
+          pre.
+
+Definition get_post (an:clause) :=
+          let (pre,post) := an in
+          post.
+
+Module Phi.
+
+  Definition phi : Type := Proc.t -> clause.
+
+  Definition empty_phi: phi := fun _ => empty_clause.
+
+End Phi.
+
+(* Defintion of a Hoare Triple with inliner*)
+
+Definition i_hoare_triple (n: nat) (P Q: assertion) (c : com) (ps : Psi.psi) : Prop :=
+  forall s s',  P s -> ceval c s (k_inliner_ps n ps) s'  -> Q s'.
+
+
+Lemma i_hoare_triple_hoare_triple :
   forall P Q p ps,
-    (hoare_triple_proc ps -> hoare_triple P Q p ps) ->
-    (hoare_triple_proc ps -> hoare_triple_body ps) ->
+  hoare_triple P Q p ps <-> forall n, i_hoare_triple n P Q p ps.
+Proof.
+unfold hoare_triple, i_hoare_triple;split;intros H.
+* intros n s s' Pre Heval.
+  eapply H.
+  apply Pre.
+  apply n_inline_ps_ceval in Heval.
+  assumption.
+* intros s s' HPre Heval.
+  apply ceval_n_inline_ps in Heval.
+  destruct Heval.
+  eapply H.
+  + apply HPre.
+  + apply H0.
+Qed.
+
+(* Hoare triple for a com  with procedure context *)
+
+Definition hoare_triple_ctx (cl : Phi.phi) (ps: Psi.psi)
+                            (P Q : assertion) (c: com) :=
+    (forall p, hoare_triple (get_pre (cl p)) (get_post (cl p)) (CCall p) ps) ->
+      hoare_triple P Q c ps.
+
+(* Hoare triple for ap procedure with the procedure context *)
+
+Definition hoare_triple_proc_ctx (cl : Phi.phi) (ps_init :Psi.psi):=
+forall p ps, hoare_triple_ctx cl ps (get_pre (cl p)) (get_post (cl p)) (ps_init p).
+
+Lemma recursive_proc ps cl:
+    hoare_triple_proc_ctx cl ps ->
+   (forall p, hoare_triple (get_pre (cl p)) (get_post (cl p)) (CCall p) ps).
+Proof.
+intros.
+apply i_hoare_triple_hoare_triple.
+intros n.
+generalize dependent p.
+induction n.
+* intros p s s' HPre Heval.
+  inversion Heval;subst.
+  apply ceval_inf_loop in H1.
+  contradiction H1.
+* intros p s s' HPre Heval.
+  apply n_inline_ps_inline in Heval.
+  eapply H.
+  + apply IHn.
+  + apply HPre.
+  + apply Heval.
+Qed.
+
+(* Verification of Hoare Triple with procedure *)
+
+Lemma recursion_hoare_triple :
+  forall P Q p ps cl,
+    hoare_triple_proc_ctx cl ps  ->
+    hoare_triple_ctx cl ps P Q p ->
     hoare_triple P Q p ps.
-
-(* Proof that one can use a verification condition generator to proof Hoare Triples *)
-
-Lemma correct :
-  forall p ps,
-  forall (P Q: assertion),
-    (forall m, P m -> tc' p m ps) ->
-    (forall m, P m -> tc p m ps Q) ->
-    (hoare_triple_proc ps -> hoare_triple P Q p ps).
 Proof.
-  intros p ps. 
-  induction p.
-  * unfold hoare_triple. intros. eapply H0. apply H2. inversion H3;subst. reflexivity.
-  * unfold hoare_triple. intros. eapply H0. apply H2. inversion H3;subst. reflexivity.
-  * unfold hoare_triple. intros. eapply H0. apply H2. 
-    apply H. apply H2. inversion H3;subst. reflexivity. 
-  * intros P Q Htc' Htc Hproc. eapply seq_hoare_triple.
-  + apply IHp1.
-  - apply Htc'.
-  - simpl in Htc', Htc.
-    intros.
-    specialize (Htc' m H).
-    destruct Htc'.
-    specialize (Htc m H). 
-    specialize 
-      (tc_split p1 ps m (fun m' : sigma => tc' p2 m' ps) (fun m' : sigma => tc p2 m' ps Q)).
-    intros.
-    apply H2. assumption. assumption.
-  - assumption.
-    + apply IHp2.
-  - intros. destruct H. assumption.
-  - intros. destruct H. assumption.
-  - assumption.
-    * intros P Q Htc' Htc Hproc. apply if_hoare_triple.
-    + apply IHp1.
-  - intros. apply Htc'. apply H. apply H.
-  - intros. simpl in Htc. destruct H. specialize (Htc m H). destruct Htc.
-    apply H1. apply bexp_eval_true. assumption.
-  - assumption.
-    + apply IHp2.
-  - intros. apply Htc'. apply H. destruct H. apply bexp_eval_false in H0. apply H0.
-  - intros. simpl in H. destruct H. specialize (Htc m H). destruct Htc.
-    apply H2. apply bexp_eval_false. assumption.
-  - assumption.
-    * intros  P Q Htc' Htc.
-      specialize (IHp (fun s => inv s /\ beval s b = true) inv).
-      intros Hproc s s' Pre.
-      apply (consequence_hoare_post _ _ P _ (fun s : sigma => inv s /\ beval s b = false)).
-    + apply (consequence_hoare_pre _ _ _ inv).  
-  - apply while_hoare_triple.
-    specialize (Htc s Pre).
-    specialize (Htc' s Pre).
-    simpl in Htc, Htc'.
-    destruct Htc'.
-    destruct H0. 
-    apply IHp.
-    ** intros.
-       apply H0.
-       destruct H2.
-       apply bexp_eval_true in H3.
-       assumption.
-    ** intros.
-       apply H1.
-       apply H2.
-    ** assumption.
-  - intros.
-    specialize (Htc' s0 H).
-    apply Htc'.
-    + intros.
-      specialize (Htc s Pre).
-      apply Htc.
-      specialize (Htc' s Pre).
-      apply Htc'.
-      apply H.
-      apply H.
-    + assumption.
-      * intros P Q Htc' Htc Hproc s s' Pre.
-        apply (consequence_hoare_post _ _ P _ (get_post (snd (ps f)))).
-    + apply (consequence_hoare_pre _ _ _ (get_pre (snd (ps f)))).
-  - apply Hproc.
-  - apply Htc'.
-    + eapply Htc.
-      apply Pre.
-      apply Htc'.
-      assumption.
-    + assumption.
-Qed.
-
-Lemma correct_proc :
-  forall ps,
-    tc_p ps ->
-    (hoare_triple_proc ps -> hoare_triple_body ps).
-Proof.
-  intros ps Htc Hproc.
-  unfold hoare_triple_body.
-  intros.
-  apply correct.
-  * apply Htc.
-  * apply Htc.
-  * assumption.
-Qed.
-
-(* Examples of proofs of Hoare Triples *)
-
-Example Hoare1 : hoare_triple (fun m => m EAX = 1) (fun m' => m' EAX = 3) plus2 Psi.empty_psi.
-Proof.
-  apply recursion_hoare_triple.
-  * apply correct.
-  + simpl;intros. auto.
-  + simpl;intros.
-    rewrite H0.
-    rewrite H.
-    simpl.
-    apply set'def.
-    reflexivity.
-    * apply correct_proc.
-      apply tc_p_empty_psi.
-Qed.
-
-Definition plus3 : com := CSeq (CAss EAX (APlus (AId EAX) (ANum 2)))
-                               (CAss EAX (APlus (AId EAX) (ANum 2))).
-
-Example Haore2 : hoare_triple (fun m => m EAX = 1) (fun m' => m' EAX = 5) plus3 Psi.empty_psi.
-Proof.
-  apply recursion_hoare_triple.
-  * apply correct.
-  + simpl;intros. auto.
-  + simpl;intros.
-    rewrite H1.
-    rewrite H0.
-    rewrite H.
-    simpl.
-    apply set'def.
-    reflexivity.
-    * apply correct_proc.
-      apply tc_p_empty_psi.
-Qed.
-
-Definition if2 : com := CIf (BEq (AId EAX) (ANum 4)) plus2 plus2.
-
-Example Hoare3 : hoare_triple (fun m => m EAX = 1) (fun m' => m' EAX = 3) if2 Psi.empty_psi .
-Proof.
-  apply recursion_hoare_triple.
-  * apply correct.
-  + simpl; intros. auto.
-  + simpl;intros.
-    destruct (beval m (BEq (AId EAX) (ANum 4))) eqn:Hcond.
-  - split;intros.
-    ** rewrite H1.
-       rewrite H.
-       apply set'def.
-       reflexivity.
-    ** apply bexp_eval_true in Hcond.
-       contradiction H0.
-  - split;intros.
-    ** apply bexp_eval_false in Hcond.
-       contradiction H0.
-    ** rewrite H1.
-       rewrite H.
-       apply set'def.
-       reflexivity.
-    * apply correct_proc.
-      apply tc_p_empty_psi.
-Qed.
-
-Definition if3 : com := CSeq (CAss EAX (APlus (AId EAX) (ANum 2)))
-                             (CSeq (CIf (BEq (AId EAX) (ANum 4)) plus2 plus2) plus2).
-
-Example Hoare4 : hoare_triple (fun m => m EAX = 1) (fun m' => m' EAX = 7) if3 Psi.empty_psi.
-Proof.
-  apply recursion_hoare_triple.
-  * apply correct.
-  + simpl;intros. auto.
-  + simpl;intros.
-    destruct (beval m' (BEq (AId EAX) (ANum 4))) eqn:Hcond.
-  - split;intros.
-    ** rewrite H3.
-       rewrite H2.
-       rewrite H0.
-       rewrite H.
-       apply set'def.
-       reflexivity.
-    ** apply bexp_eval_true in Hcond.
-       contradiction H1.
-  - split;intros.
-    ** apply bexp_eval_false in Hcond.
-       contradiction H1.
-    ** rewrite H3.
-       rewrite H2.
-       rewrite H0.
-       rewrite H.
-       apply set'def.
-       reflexivity.
-    * apply correct_proc.
-      apply tc_p_empty_psi.
-Qed.
-
-Definition assert3 : com := CSeq (CAssert (fun m => m EAX = 2))
-                                 (CAssert (fun m => m EAX = 2)).
-
-Example Hoare6 : hoare_triple (fun m => m EAX = 2) (fun _ => True) assert3 Psi.empty_psi.
-Proof.
-  apply recursion_hoare_triple.
-  * apply correct.
-  + simpl;intros.
-    split.
-  - assumption.
-  - intros.
-    rewrite <- H1.
-    assumption.
-    + simpl; intros. auto.
-      * apply correct_proc.
-        apply tc_p_empty_psi.
-Qed.
-
-Definition if4 : com := CIf (BEq (AId EAX) (ANum 2)) (CAssert (fun m => m EAX = 2)) CSkip.
-
-Example Hoare7 : hoare_triple (fun m => m EAX = 2) (fun m' => m' EAX = 2) if4 Psi.empty_psi.
-Proof.
-  apply recursion_hoare_triple.
-  * apply correct.
-  + simpl;intros. 
-    split.
-  - intros.
-    assumption.
-  - auto.
-    + simpl;intros.
-      destruct (beval m (BEq (AId EAX) (ANum 2))) eqn:Hcond.
-  - split;intros.
-    ** rewrite <- H2.
-       assumption.
-    ** apply bexp_eval_true in Hcond.
-       contradiction H0.
-  - split;intros.
-    ** apply bexp_eval_false in Hcond.
-       contradiction H0.
-    ** rewrite <- H1.
-       assumption.
-    * apply correct_proc.
-      apply tc_p_empty_psi.
+intros.
+apply H0.
+apply recursive_proc.
+assumption.
 Qed.
