Vcg_Opt.v
@@ -4,14 +4,15 @@ From Rela Require Import Com.
 From Rela Require Import Proc.
 From Rela Require Import Sigma.
 From Rela Require Import Loc.
-From Rela Require Import Vcg.
+From Rela Require Vcg.
+From Rela Require Import Hoare_Triple.
 
-Import Why3_Set.
+Import Vcg.Why3_Set.
+Import Vcg.Assn_b.
 
-Inductive branch (A B C : Prop) : Prop :=  
+Inductive branch (A B C : Prop) : Prop :=
   | Then : A -> B -> branch A B C
   | Else : ~ A -> C -> branch A B C.
-
 
 Lemma branch_simpl : forall A B C,
 branch A B C -> (A -> B) /\ (~A -> C).
@@ -26,40 +27,30 @@ destruct H.
   * auto.
 Qed.
 
-
 Fixpoint tc (c : com) (m : Sigma.sigma)
-            (ps: Psi.psi) (suite : Sigma.sigma -> Prop) : Prop :=
+            (cl: Phi.phi) (suite : Sigma.sigma -> Prop) : Prop :=
     match c with
     | CSkip => forall m', m = m' -> suite m'
     | CAss x a => forall m', (m' = set m x (aeval m a)) -> suite m'
     | CAssert b => forall m', b m -> m = m' -> suite m'
-    | CSeq p1 p2 => tc p1 m ps (fun m' => tc p2 m' ps suite)
+    | CSeq p1 p2 => tc p1 m cl (fun m' => tc p2 m' cl suite)
     | CIf b p1 p2 =>
-               tc p1 m ps (fun m1' => 
-               tc p2 m ps (fun m2' => 
+               tc p1 m cl (fun m1' =>
+               tc p2 m cl (fun m2' =>
                forall m',
                branch (bassn b m) (m' = m1') (m' = m2') -> suite m'))
-    (*| CWhile b p inv _ => inv m -> inv m' -> beval m b = false -> suite *)
-    end.
-
-Fixpoint tc' (c : com) (m : Sigma.sigma)
-            (ps: Psi.psi) : Prop :=
-    match c with
-    | CSkip => True
-    | CAss x a => True
-    | CAssert b => b m 
-    | CSeq p1 p2 => tc' p1 m ps /\
-                    tc p1 m ps (fun m' => tc' p2 m' ps)
-    | CIf b p1 p2 => 
-      (bassn b m -> tc' p1 m ps) /\ (~bassn b m -> tc' p2 m ps)
+    | CWhile b p inv => inv m ->
+                        forall m', inv m' -> beval m' b = false -> suite m'
+    | CCall f => (get_pre (cl f)) m ->
+                  forall m',  (get_post (cl f)) m' -> suite m'
     end.
 
 Lemma consequence_tc_suite :
-forall p ps m (suite1 suite2 : Sigma.sigma -> Prop),
+forall p cl m (suite1 suite2 : Sigma.sigma -> Prop),
 (forall s, suite1 s -> suite2 s) ->
-tc p m ps suite1 -> tc p m ps suite2.
+tc p m cl suite1 -> tc p m cl suite2.
 Proof.
-intros p ps.
+intros p cl.
 induction p.
   * intros. simpl. simpl in H0.
     intros.
@@ -93,12 +84,20 @@ induction p.
         generalize H3. generalize m'. apply H2.
        + apply H1. 
      - apply H0.
+  * intros. simpl. simpl in H0.
+    intros. apply H.
+    apply H0.
+    all : try assumption.
+  * intros. simpl. simpl in H0.
+    intros. apply H.
+    apply H0.
+    all : try assumption.
 Qed.
 
 Lemma split_tc :
-forall p m ps (suite1 suite2 : Sigma.sigma -> Prop),
-tc p m ps (fun m' => suite1 m' /\ suite2 m') ->
-tc p m ps suite1 /\ tc p m ps suite2.
+forall p m cl (suite1 suite2 : Sigma.sigma -> Prop),
+tc p m cl (fun m' => suite1 m' /\ suite2 m') ->
+tc p m cl suite1 /\ tc p m cl suite2.
 Proof.
 intros.
 split.
@@ -115,15 +114,15 @@ split.
 Qed.
 
 Lemma opt_1_true:
-forall p1 p2 b m ps (suite : Sigma.sigma -> Prop),
+forall p1 p2 b m cl (suite : Sigma.sigma -> Prop),
 bassn b m ->
-tc p1 m ps (fun m1' => 
-tc p2 m ps (fun m2' =>  forall m', branch (bassn b m) (m' = m1') (m' = m2') -> suite m')) ->
-tc p1 m ps (fun m1' => 
-tc p2 m ps (fun m2' =>  forall m', m' = m1' -> suite m')).
+tc p1 m cl (fun m1' => 
+tc p2 m cl (fun m2' =>  forall m', branch (bassn b m) (m' = m1') (m' = m2') -> suite m')) ->
+tc p1 m cl (fun m1' => 
+tc p2 m cl (fun m2' =>  forall m', m' = m1' -> suite m')).
 Proof.
 intros.
-apply (consequence_tc_suite _ _ _ (fun m1' => tc p2 m ps (fun m2' => forall m', branch (bassn b m) (m' = m1') (m' = m2') -> suite m'))).
+apply (consequence_tc_suite _ _ _ (fun m1' => tc p2 m cl (fun m2' => forall m', branch (bassn b m) (m' = m1') (m' = m2') -> suite m'))).
 * intros.
   apply (consequence_tc_suite _ _ _ (fun m2' : sigma => forall m' : sigma, branch (bassn b m) (m' = s) (m' = m2') -> suite m')).
   -  intros. apply H2.
@@ -135,15 +134,15 @@ apply (consequence_tc_suite _ _ _ (fun m1' => tc p2 m ps (fun m2' => forall m', 
 Qed.
 
 Lemma opt_1_false:
-forall p1 p2 b m ps (suite : Sigma.sigma -> Prop),
+forall p1 p2 b m cl (suite : Sigma.sigma -> Prop),
 ~bassn b m ->
-tc p1 m ps (fun m1' => 
-tc p2 m ps (fun m2' =>  forall m', branch (bassn b m) (m' = m1') (m' = m2') -> suite m')) ->
-tc p1 m ps (fun m1' => 
-tc p2 m ps (fun m2' =>  forall m', m' = m2' -> suite m')).
+tc p1 m cl (fun m1' => 
+tc p2 m cl (fun m2' =>  forall m', branch (bassn b m) (m' = m1') (m' = m2') -> suite m')) ->
+tc p1 m cl (fun m1' => 
+tc p2 m cl (fun m2' =>  forall m', m' = m2' -> suite m')).
 Proof.
 intros.
-apply (consequence_tc_suite _ _ _ (fun m1' => tc p2 m ps (fun m2' => forall m', branch (bassn b m) (m' = m1') (m' = m2') -> suite m'))).
+apply (consequence_tc_suite _ _ _ (fun m1' => tc p2 m cl (fun m2' => forall m', branch (bassn b m) (m' = m1') (m' = m2') -> suite m'))).
 * intros.
   apply (consequence_tc_suite _ _ _ (fun m2' : sigma => forall m' : sigma, branch (bassn b m) (m' = s) (m' = m2') -> suite m')).
   -  intros. apply H2.
@@ -155,15 +154,15 @@ apply (consequence_tc_suite _ _ _ (fun m1' => tc p2 m ps (fun m2' => forall m', 
 Qed.
 
 Lemma opt_2_true:
-forall p1 p2 m ps (suite : Sigma.sigma -> Prop),
-tc p1 m ps (fun m1' => 
-tc p2 m ps (fun m2' =>  forall m',  m' = m1' -> suite m')) ->
-tc p1 m ps (fun m1' => 
-tc p2 m ps (fun m2' =>  suite m1')).
+forall p1 p2 m cl (suite : Sigma.sigma -> Prop),
+tc p1 m cl (fun m1' => 
+tc p2 m cl (fun m2' =>  forall m',  m' = m1' -> suite m')) ->
+tc p1 m cl (fun m1' => 
+tc p2 m cl (fun m2' =>  suite m1')).
 Proof.
 intros.
 apply (consequence_tc_suite _ _ _ (fun m1' => 
-                                      tc p2 m ps (fun m2' =>  forall m',  m' = m1'-> suite m'))).
+                                      tc p2 m cl (fun m2' =>  forall m',  m' = m1'-> suite m'))).
   + intros.
     eapply consequence_tc_suite in H0.
     - apply H0.
@@ -174,15 +173,15 @@ apply (consequence_tc_suite _ _ _ (fun m1' =>
 Qed.
 
 Lemma opt_2_false:
-forall p1 p2 m ps (suite : Sigma.sigma -> Prop),
-tc p1 m ps (fun m1' => 
-tc p2 m ps (fun m2' =>  forall m',  m' = m2' -> suite m')) ->
-tc p1 m ps (fun m1' => 
-tc p2 m ps (fun m2' =>  suite m2')).
+forall p1 p2 m cl (suite : Sigma.sigma -> Prop),
+tc p1 m cl (fun m1' => 
+tc p2 m cl (fun m2' =>  forall m',  m' = m2' -> suite m')) ->
+tc p1 m cl (fun m1' => 
+tc p2 m cl (fun m2' =>  suite m2')).
 Proof.
 intros.
 apply (consequence_tc_suite _ _ _ (fun m1' => 
-                                      tc p2 m ps (fun m2' =>  forall m',  m' = m2'-> suite m'))).
+                                      tc p2 m cl (fun m2' =>  forall m',  m' = m2'-> suite m'))).
   + intros.
     eapply consequence_tc_suite in H0.
     - apply H0.
@@ -193,11 +192,11 @@ apply (consequence_tc_suite _ _ _ (fun m1' =>
 Qed.
 
 Lemma tc_split :
-forall p ps m (suite1 suite2 : Sigma.sigma -> Prop),
-tc p m ps suite1 -> tc p m ps suite2 ->
-tc p m ps (fun m' => suite1 m' /\ suite2 m').
+forall p cl m (suite1 suite2 : Sigma.sigma -> Prop),
+tc p m cl suite1 -> tc p m cl suite2 ->
+tc p m cl (fun m' => suite1 m' /\ suite2 m').
 Proof.
-intros p ps.
+intros p cl.
 induction p.
 + simpl. intros.
   split.
@@ -212,7 +211,7 @@ induction p.
   apply H. assumption. subst. reflexivity.
   apply H0. assumption. subst. reflexivity.
 + simpl. intros.
-  apply (consequence_tc_suite _ _ _ (fun m => tc p2 m ps suite1 /\ tc p2 m ps suite2)).
+  apply (consequence_tc_suite _ _ _ (fun m => tc p2 m cl suite1 /\ tc p2 m cl suite2)).
   * intros. destruct H1. apply IHp2. assumption. assumption.
   * apply IHp1. assumption. assumption.
 + intros.
@@ -225,13 +224,13 @@ induction p.
     apply opt_2_true in H.
     apply opt_2_true in H0.
     apply (consequence_tc_suite _ _ _ 
-        (fun m' => tc p2 m ps ( fun _ => suite1 m' /\ suite2 m'))).
+        (fun m' => tc p2 m cl ( fun _ => suite1 m' /\ suite2 m'))).
         - intros s. apply consequence_tc_suite.
           intros. destruct H3.
           ++ subst. assumption.
           ++ contradiction H3.
         - apply (consequence_tc_suite _ _ _ 
-        (fun m' => tc p2 m ps ( fun _ => suite1 m') /\ tc p2 m ps ( fun _ => suite2 m'))).
+        (fun m' => tc p2 m cl ( fun _ => suite1 m') /\ tc p2 m cl ( fun _ => suite2 m'))).
           ++ intros.  destruct H2. apply IHp2. assumption. assumption.
           ++ apply IHp1. assumption. assumption.
         - assumption.
@@ -243,26 +242,57 @@ induction p.
     apply opt_2_false in H.
     apply opt_2_false in H0.
     apply (consequence_tc_suite _ _ _ 
-        (fun _ => tc p2 m ps ( fun m' => suite1 m' /\ suite2 m'))).
+        (fun _ => tc p2 m cl ( fun m' => suite1 m' /\ suite2 m'))).
         - intros s. apply consequence_tc_suite.
           intros. destruct H3.
           ++ contradiction H3.
           ++ subst. assumption.
         - apply (consequence_tc_suite _ _ _ 
-        (fun _ => tc p2 m ps ( fun m' => suite1 m') /\ tc p2 m ps ( fun m' => suite2 m'))).
+        (fun _ => tc p2 m cl ( fun m' => suite1 m') /\ tc p2 m cl ( fun m' => suite2 m'))).
           ++ intros.  destruct H2. apply IHp2. assumption. assumption.
           ++ apply IHp1. assumption. assumption.
         - assumption.
         - assumption.
++ simpl. intros.
+  split. 
+    * apply H.
+      all: try assumption.
+    * apply H0.
+      all: try assumption.
++ simpl. intros.
+  split.
+    * apply H.
+      all: try assumption.
+    * apply H0.
+      all: try assumption.
 Qed.
 
+Fixpoint tc' (c : com) (m : Sigma.sigma)
+            (cl: Phi.phi) : Prop :=
+    match c with
+    | CSkip => True
+    | CAss x a => True
+    | CAssert b => b m
+    | CSeq p1 p2 => tc' p1 m cl /\
+                    tc p1 m cl (fun m' => tc' p2 m' cl)
+    | CIf b p1 p2 =>
+      (bassn b m -> tc' p1 m cl) /\ (~bassn b m -> tc' p2 m cl)
+   | CWhile b p inv => inv m /\
+                          (forall m', bassn b m' -> tc' p m' cl) /\
+                          (forall m', inv m'  -> tc p m' cl inv)
+   | CCall f => (get_pre (cl f)) m
+    end.
+
+Definition tc_p (ps: Psi.psi) (cl : Phi.phi) : Prop :=
+    forall f m, (get_pre (cl f)) m -> tc' (ps f) m cl /\
+                tc (ps f) m cl (get_post (cl f)).
 
   (* use relational properties : module Opt to an proper file*)
 
 (*Lemma simpl_tc :
-forall p ps suite, forall m, tc p m ps (fun _ => suite) -> suite.
+forall p cl suite, forall m, tc p m cl (fun _ => suite) -> suite.
 Proof.
-intros p ps suite.
+intros p cl suite.
 induction p.
 * simpl in H. specialize (H m). apply H. reflexivity.
 * simpl in H. specialize (H (set m x (aeval m a))). apply H. reflexivity.
@@ -270,10 +300,10 @@ induction p.
 * simpl in H, H0.
   destruct H.
    specialize 
-    (tc_split p1 ps m (fun m' : sigma => tc' p2 m' ps) (fun m' : sigma => tc p2 m' ps (fun _ : sigma => suite))).
+    (tc_split p1 cl m (fun m' : sigma => tc' p2 m' cl) (fun m' : sigma => tc p2 m' cl (fun _ : sigma => suite))).
      intros.
      specialize (H2 H1 H0).
-  eapply (consequence_tc_suite _ _ _ _ (fun m' : sigma => tc' p2 m' ps /\suite)) in H2.
+  eapply (consequence_tc_suite _ _ _ _ (fun m' : sigma => tc' p2 m' cl /\suite)) in H2.
   + apply split_tc in H2.
     destruct H2.
     eapply IHp1.
@@ -310,108 +340,3 @@ Qed.*)
 *)
 
 
-(* --------------------  Move two Hoare module -------------------------------  *)
-
-
-Lemma test1 : forall m,  m EAX = 1 -> tc plus2 m Psi.empty_psi (fun m' => m' EAX = 3) .
-Proof.
-simpl.
-intros.
-rewrite H0.
-rewrite H.
-simpl.
-apply set'def.
-reflexivity.
-Qed.
-
-Definition plus3 : com := CSeq (CAss EAX (APlus (AId EAX) (ANum 2)))
-                                (CAss EAX (APlus (AId EAX) (ANum 2))).
-
-Lemma test2 : forall m , m EAX = 1 -> tc plus3 m Psi.empty_psi (fun m' => m' EAX = 5).
-Proof.
-simpl.
-intros.
-rewrite H1.
-rewrite H0.
-rewrite H.
-simpl.
-apply set'def.
-reflexivity.
-Qed.
-
-Definition if2 : com := CIf (BEq (AId EAX) (ANum 4)) plus2 plus2.
-
-Lemma test3 : forall m, m EAX = 1 -> tc if2 m Psi.empty_psi (fun m' => m' EAX = 3).
-Proof.
-simpl.
- intros.
- destruct H2.
- + rewrite H3.
-   rewrite H0.
-   rewrite H.
-   apply set'def.
-   reflexivity.
- + rewrite H3.
-   rewrite H1.
-   rewrite H.
-   apply set'def.
-   reflexivity.
-Qed.
-
-Definition if3 : com := CSeq (CAss EAX (APlus (AId EAX) (ANum 2)))
-                            (CSeq (CIf (BEq (AId EAX) (ANum 4)) plus2 plus2) plus2).
-
-Lemma test4 : forall m, m EAX = 1 -> tc if3 m Psi.empty_psi (fun m' => m' EAX = 7).
-Proof.
- simpl.
-  intros.
-  rewrite H4.
-  destruct H3.
-  * rewrite H5.
-    rewrite H1.
-    rewrite H0.
-    rewrite H.
-    apply set'def.
-    reflexivity.
-  * rewrite H5.
-    rewrite H2.
-    rewrite H0.
-    rewrite H.
-    apply set'def.
-    reflexivity.
-Qed.
-
-Lemma test5 : forall m1 m2, m1 EAX = m2 EAX -> 
-                              tc plus2 m1 Psi.empty_psi ( fun m1' => tc plus2 m2 Psi.empty_psi (fun m2' => m1' EAX = m2' EAX)).
-Proof.
-  simpl.
-  intros.
-  rewrite H1.
-  rewrite H0.
-  rewrite H.
-  apply set'def.
-  reflexivity.
-Qed.
-
-Definition truc3 : com := CSeq (CAssert (fun m => m EAX = 2))
-                          (CAssert (fun m => m EAX = 2)).
-
-Lemma test6 : forall m, (m EAX = 2) -> tc' truc3 m  Psi.empty_psi.
-Proof.
-intros.
-simpl.
-split. 
-  * assumption.
-  * intros. rewrite <- H1. assumption.
-Qed.
-
-Definition if4 : com := CIf (BEq (AId EAX) (ANum 2)) (CAssert (fun m => m EAX = 2)) CSkip.
-
-Lemma test7 : forall m, (m EAX = 2) -> tc' if4 m  Psi.empty_psi.
-Proof.
-intros.
-simpl.
-split. 
-  * auto.
-  * auto.
-Qed.
