Correct.v
@@ -1,0 +1,253 @@
+From Rela Require Import Vcg.
+From Rela Require Import Hoare_Triple.
+From Rela Require Import Com.
+From Rela Require Import Aexp.
+From Rela Require Import Bexp.
+From Rela Require Import Sigma.
+From Rela Require Import Loc.
+Import Why3_Set.
+Import Assn_b.
+
+(** Proof that one can use a verification condition generator to proof Hoare Triples **)
+
+Lemma correct :
+  forall p cl ps,
+  forall (P Q: assertion),
+    (forall m, P m -> tc' p m cl) ->
+    (forall m, P m -> tc p m cl Q) ->
+    hoare_triple_ctx cl ps P Q p.
+Proof.
+  unfold hoare_triple_ctx.
+  intros p cl ps.
+  induction p.
+  * unfold hoare_triple. intros. eapply H0. apply H2. inversion H3;subst. reflexivity.
+  * unfold hoare_triple. intros. eapply H0. apply H2. inversion H3;subst. reflexivity.
+  * unfold hoare_triple. intros. eapply H0. apply H2.
+    apply H. apply H2. inversion H3;subst. reflexivity.
+  * intros P Q Htc' Htc Hproc. eapply seq_hoare_triple.
+  + apply IHp1.
+  - apply Htc'.
+  - simpl in Htc', Htc.
+    intros.
+    specialize (Htc' m H).
+    destruct Htc'.
+    specialize (Htc m H).
+    specialize
+      (tc_split p1 cl m
+                (fun m' : sigma => tc' p2 m' cl) (fun m' : sigma => tc p2 m' cl Q)).
+    intros.
+    apply H2. assumption. assumption.
+  - assumption.
+    + apply IHp2.
+  - intros. destruct H. assumption.
+  - intros. destruct H. assumption.
+  - assumption.
+    * intros P Q Htc' Htc Hproc. apply if_hoare_triple.
+    + apply IHp1.
+  - intros. apply Htc'. apply H. apply H.
+  - intros. simpl in Htc. destruct H. specialize (Htc m H). destruct Htc.
+    apply H1. apply bexp_eval_true. assumption.
+  - assumption.
+    + apply IHp2.
+  - intros. apply Htc'. apply H. destruct H. apply bexp_eval_false in H0. apply H0.
+  - intros. simpl in H. destruct H. specialize (Htc m H). destruct Htc.
+    apply H2. apply bexp_eval_false. assumption.
+  - assumption.
+    * intros  P Q Htc' Htc.
+      specialize (IHp (fun s => inv s /\ beval s b = true) inv).
+      intros Hproc s s' Pre.
+      apply
+        (consequence_hoare_post _ _ P _ (fun s : sigma => inv s /\ beval s b = false)).
+    + apply (consequence_hoare_pre _ _ _ inv).
+  - apply while_hoare_triple.
+    specialize (Htc s Pre).
+    specialize (Htc' s Pre).
+    simpl in Htc, Htc'.
+    destruct Htc'.
+    destruct H0.
+    apply IHp.
+    ** intros.
+       apply H0.
+       destruct H2.
+       apply bexp_eval_true in H3.
+       assumption.
+    ** intros.
+       apply H1.
+       apply H2.
+    ** assumption.
+  - intros.
+    specialize (Htc' s0 H).
+    apply Htc'.
+    + intros.
+      specialize (Htc s Pre).
+      apply Htc.
+      specialize (Htc' s Pre).
+      apply Htc'.
+      apply H.
+      apply H.
+    + assumption.
+ * intros P Q Htc' Htc Hproc.
+  intros s s' Pre.
+   apply (consequence_hoare_post _ _ P _ (get_post (cl f))).
+    + apply (consequence_hoare_pre _ _ _ (get_pre (cl f))).
+      - apply Hproc.
+      - apply Htc'.
+    + eapply Htc.
+      apply Pre.
+      apply Htc'.
+      assumption.
+    + assumption.
+Qed.
+
+Lemma correct_proc :
+  forall cl ps,
+    tc_p cl ps ->
+    hoare_triple_proc_ctx ps cl.
+Proof.
+  intros cl ps Htc.
+  unfold hoare_triple_proc_ctx.
+  intros.
+  apply correct.
+  * apply Htc.
+  * apply Htc.
+Qed.
+
+(** Examples of proofs of Hoare Triples **)
+
+Example Hoare1 : hoare_triple (fun m => m EAX = 1) (fun m' => m' EAX = 3) plus2 Psi.empty_psi.
+Proof.
+apply recursion_hoare_triple with Phi.empty_phi.
+* apply correct_proc.
+  apply tc_p_empty_psi.
+* apply correct.
+  + simpl;intros. auto.
+  + simpl;intros.
+    rewrite H0.
+    rewrite H.
+    simpl.
+    apply set'def.
+    reflexivity.
+Qed.
+
+Definition plus3 : com := CSeq (CAss EAX (APlus (AId EAX) (ANum 2)))
+                               (CAss EAX (APlus (AId EAX) (ANum 2))).
+
+Example Haore2 : hoare_triple (fun m => m EAX = 1) (fun m' => m' EAX = 5) plus3 Psi.empty_psi.
+Proof.
+apply recursion_hoare_triple with Phi.empty_phi.
+* apply correct_proc.
+  apply tc_p_empty_psi.
+* apply correct.
+  + simpl;intros. auto.
+  + simpl;intros.
+    rewrite H1.
+    rewrite H0.
+    rewrite H.
+    simpl.
+    apply set'def.
+    reflexivity.
+Qed.
+
+Definition if2 : com := CIf (BEq (AId EAX) (ANum 4)) plus2 plus2.
+
+Example Hoare3 : hoare_triple (fun m => m EAX = 1) (fun m' => m' EAX = 3) if2 Psi.empty_psi .
+Proof.
+apply recursion_hoare_triple with Phi.empty_phi.
+* apply correct_proc.
+  apply tc_p_empty_psi.
+* apply correct.
+  + simpl; intros. auto.
+  + simpl;intros.
+    destruct (beval m (BEq (AId EAX) (ANum 4))) eqn:Hcond.
+    - split;intros.
+      ** rewrite H1.
+         rewrite H.
+         apply set'def.
+         reflexivity.
+      ** apply bexp_eval_true in Hcond.
+         contradiction H0.
+    - split;intros.
+      ** apply bexp_eval_false in Hcond.
+         contradiction H0.
+      ** rewrite H1.
+         rewrite H.
+         apply set'def.
+         reflexivity.
+Qed.
+
+Definition if3 : com := CSeq (CAss EAX (APlus (AId EAX) (ANum 2)))
+                             (CSeq (CIf (BEq (AId EAX) (ANum 4)) plus2 plus2) plus2).
+
+Example Hoare4 : hoare_triple (fun m => m EAX = 1) (fun m' => m' EAX = 7) if3 Psi.empty_psi.
+Proof.
+apply recursion_hoare_triple with Phi.empty_phi.
+* apply correct_proc.
+  apply tc_p_empty_psi.
+* eapply correct.
+  + simpl;intros. auto.
+  + simpl;intros.
+    destruct (beval m' (BEq (AId EAX) (ANum 4))) eqn:Hcond.
+    - split;intros.
+      ** rewrite H3.
+         rewrite H2.
+         rewrite H0.
+         rewrite H.
+         apply set'def.
+         reflexivity.
+      ** apply bexp_eval_true in Hcond.
+         contradiction H1.
+    - split;intros.
+      ** apply bexp_eval_false in Hcond.
+         contradiction H1.
+      ** rewrite H3.
+         rewrite H2.
+         rewrite H0.
+         rewrite H.
+         apply set'def.
+         reflexivity.
+Qed.
+
+Definition assert3 : com := CSeq (CAssert (fun m => m EAX = 2))
+                                 (CAssert (fun m => m EAX = 2)).
+
+Example Hoare6 : hoare_triple (fun m => m EAX = 2) (fun _ => True) assert3 Psi.empty_psi.
+Proof.
+apply recursion_hoare_triple with Phi.empty_phi.
+* apply correct_proc.
+  apply tc_p_empty_psi.
+* apply correct.
+  + simpl;intros.
+    split.
+    - assumption.
+    - intros.
+      rewrite <- H1.
+      assumption.
+  + simpl; intros. auto.
+Qed.
+
+Definition if4 : com := CIf (BEq (AId EAX) (ANum 2)) (CAssert (fun m => m EAX = 2)) CSkip.
+
+Example Hoare7 : hoare_triple (fun m => m EAX = 2) (fun m' => m' EAX = 2) if4 Psi.empty_psi.
+Proof.
+apply recursion_hoare_triple with Phi.empty_phi.
+* apply correct_proc.
+  apply tc_p_empty_psi.
+* apply correct.
+  + simpl;intros.
+    split.
+    - intros.
+      assumption.
+    - auto.
+  + simpl;intros.
+    destruct (beval m (BEq (AId EAX) (ANum 2))) eqn:Hcond.
+    - split;intros.
+      ** rewrite <- H2.
+         assumption.
+      ** apply bexp_eval_true in Hcond.
+         contradiction H0.
+    - split;intros.
+      ** apply bexp_eval_false in Hcond.
+         contradiction H0.
+      ** rewrite <- H1.
+         assumption.
+Qed.
