Inliner.v
@@ -1,0 +1,581 @@
+From Rela Require Import Com.
+From Rela Require Import Loc.
+From Rela Require Import Aexp.
+From Rela Require Import Bexp.
+From Rela Require Import Proc.
+From Rela Require Import Sigma.
+
+(** Function for procedure inlining in Com **)
+
+Fixpoint inliner c inline :=
+  match c with
+  | CSeq p1 p2 => CSeq (inliner p1 inline) (inliner p2 inline)
+  | CIf b p1 p2 => CIf b (inliner p1 inline) (inliner p2 inline)
+  | CWhile b p inv => CWhile b (inliner p inline) inv
+  | CCall f => inline f
+  | _ => c
+end.
+
+(** Function for recursive procedure inlining in Com **)
+
+Fixpoint k_inliner n c (ps : Psi.psi) :=
+  match n with
+  | 0 => CWhile BTrue CSkip (fun _ => True)
+  | S n' => inliner c (fun f => k_inliner n' (ps f) ps)
+end.
+
+(** Function for procedure inlining in Psi.psi **)
+
+Definition k_inliner_ps n ps := fun p => k_inliner n (ps p) ps.
+
+(** Some fact about the inlining **)
+
+Lemma inline_cskip n ps : k_inliner (S n) CSkip ps = CSkip.
+Proof.
+ reflexivity.
+Qed.
+
+Lemma inline_cass n ps x a1: k_inliner (S n) (CAss x a1) ps = (CAss x a1).
+Proof.
+ reflexivity.
+Qed.
+
+Lemma inline_cassert n ps b: k_inliner (S n) (CAssert b) ps = (CAssert b).
+Proof.
+ reflexivity.
+Qed.
+
+Lemma inline_cseq n ps p1 p2: k_inliner (S n) (CSeq p1 p2) ps =
+                              CSeq (k_inliner (S n) p1 ps) (k_inliner (S n) p2 ps).
+Proof.
+ reflexivity.
+Qed.
+
+Lemma inline_cif n ps b p1 p2: k_inliner (S n) (CIf b p1 p2) ps =
+                               CIf b (k_inliner (S n)  p1 ps) (k_inliner (S n) p2 ps).
+Proof.
+ reflexivity.
+Qed.
+
+Lemma inline_cwhile n ps p b inv: k_inliner (S n) (CWhile b p inv) ps =
+                                  CWhile b (k_inliner (S n) p ps) inv.
+Proof.
+ reflexivity.
+Qed.
+
+Lemma inline_ccall n f ps :
+   k_inliner (S n) (CCall f) ps = k_inliner n (ps f) ps.
+Proof.
+ reflexivity.
+Qed.
+
+(* ceval is inlining insensitive on command *)
+
+Lemma ceval_inline p s ps s':
+  ceval p s ps s' -> ceval (inliner p ps) s ps s'.
+Proof.
+intros.
+induction H.
+  + apply E_Skip.
+  + apply E_Ass.
+    now auto.
+  + apply E_Assert.
+    now auto.
+  + simpl. apply E_IfTrue; [now auto | now auto].
+  + simpl. apply E_IfFalse; [now auto | now auto].
+  + simpl. eapply E_Seq.
+    - apply IHceval1.
+    - apply IHceval2.
+  + apply E_WhileFalse; now auto.
+  + simpl. eapply E_WhileTrue; [now auto | | ].
+    - apply IHceval1.
+    - apply IHceval2.
+  + simpl. assumption.
+Qed.
+
+Lemma inline_ceval p s ps s':
+  ceval (inliner p ps) s ps s' -> ceval p s ps s'.
+Proof.
+intros.
+generalize dependent s.
+generalize dependent s'.
+generalize dependent ps.
+induction p;intros.
+  + inversion H;subst.
+    apply E_Skip.
+  + inversion H;subst.
+    apply E_Ass. now auto.
+  + inversion H;subst.
+    apply E_Assert. now auto.
+  + inversion H;subst.
+    eapply E_Seq.
+    * apply IHp1. apply H2.
+    * apply IHp2. apply H6.
+  + inversion H;subst.
+    * eapply E_IfTrue.
+      assumption.
+      apply IHp1. apply H7.
+    * eapply E_IfFalse.
+      assumption.
+      apply IHp2. apply H7.
+   + remember (inliner (CWhile b p inv) ps) as original_command eqn:Horig.
+     induction H.
+     * inversion Horig.
+     * inversion Horig.
+     * inversion Horig.
+     * inversion Horig.
+     * inversion Horig.
+     * inversion Horig.
+     * inversion Horig;subst.
+       eapply E_WhileFalse.
+       assumption.
+     * inversion Horig;subst.
+       eapply E_WhileTrue.
+       assumption.
+       apply IHp. apply H0.
+       apply IHceval2.
+       assumption.
+     * inversion Horig;subst.
+   + apply E_Call.
+      simpl in H. assumption.
+Qed.
+
+(* Inlinig on Com "n+1" times is equivalent to inline on Psi.psi "n" times *)
+
+Lemma n_inline_n_inline_ps n p s ps_init s' :
+   (forall ps, ceval (k_inliner (S n) p ps_init) s ps s') ->
+   ceval p s (k_inliner_ps n ps_init) s'.
+Proof.
+intros.
+specialize (H (k_inliner_ps n ps_init)).
+generalize dependent s.
+generalize dependent s'.
+induction p ;intros.
+* rewrite inline_cskip in H.
+  apply H.
+* rewrite inline_cass in H.
+  apply H.
+* rewrite inline_cassert in H.
+  apply H.
+* rewrite inline_cseq in H.
+  inversion H;subst.
+  apply E_Seq with s'0.
+  + apply IHp1.
+    apply H2.
+  + apply IHp2.
+    apply H6.
+* rewrite inline_cif in H.
+  inversion H;subst.
+  + apply E_IfTrue.
+    - assumption.
+    - apply IHp1.
+      apply H7.
+  + apply E_IfFalse.
+    - assumption.
+    - apply IHp2.
+      apply H7.
+* remember (k_inliner (S n) (CWhile b p inv) ps_init) as original_command eqn:Horig.
+  induction H;rewrite inline_cwhile in Horig.
+  + inversion Horig.
+  + inversion Horig.
+  + inversion Horig.
+  + inversion Horig.
+  + inversion Horig.
+  + inversion Horig.
+  + inversion Horig;subst.
+     eapply E_WhileFalse.
+     assumption.
+  + inversion Horig;subst.
+    eapply E_WhileTrue.
+    - assumption.
+    - apply IHp. apply H0.
+    - apply IHceval2.
+      assumption.
+      rewrite <- inline_cwhile in Horig.
+      apply Horig.
+  + inversion Horig;subst.
+* apply E_Call.
+  rewrite inline_ccall in H.
+  apply H.
+Qed.
+
+Lemma inline_p_ps n p ps s s' ps1 ps2:
+ceval (k_inliner n p ps) s ps1 s' ->
+ceval (k_inliner n p ps) s ps2 s'.
+Proof.
+intros.
+generalize dependent s.
+generalize dependent s'.
+generalize dependent p.
+induction n.
+* intros.
+  apply ceval_inf_loop in H.
+  contradiction H.
+* induction p;intros.
+  + inversion H;subst.
+    apply E_Skip.
+  + inversion H;subst.
+    apply E_Ass.
+    auto.
+  + inversion H;subst.
+    apply E_Assert.
+    auto.
+  + rewrite inline_cseq.
+    rewrite inline_cseq in H.
+    inversion H;subst.
+    apply E_Seq with s'0.
+    - apply IHp1.
+      apply H2.
+    - apply IHp2.
+      apply H6.
+  + rewrite inline_cif.
+    rewrite inline_cif in H.
+    inversion H;subst.
+    - apply E_IfTrue.
+      assumption.
+      apply IHp1.
+      apply H7.
+    - apply E_IfFalse.
+      assumption.
+      apply IHp2.
+      apply H7.
+  + remember (k_inliner (S n) (CWhile b p inv) ps) as original_command eqn:Horig.
+    induction H;rewrite inline_cwhile in Horig.
+    - inversion Horig.
+    - inversion Horig.
+    - inversion Horig.
+    - inversion Horig.
+    - inversion Horig.
+    - inversion Horig.
+    - inversion Horig;subst.
+      eapply E_WhileFalse.
+      assumption.
+    - inversion Horig;subst.
+      eapply E_WhileTrue.
+      ** assumption.
+      ** apply IHp. apply H0.
+      ** apply IHceval2.
+         assumption.
+         assumption.
+         rewrite <- inline_cwhile in Horig.
+         apply Horig.
+     - inversion Horig;subst.
+  + apply IHn.
+    apply H.
+Qed.
+
+Lemma n_ps_inline_n_inline n p s ps_init s' :
+   ceval p s (k_inliner_ps n ps_init) s' ->
+   (forall ps, ceval (k_inliner (S n) p ps_init) s ps s').
+Proof.
+intros.
+generalize dependent s.
+generalize dependent s'.
+induction p;intros.
+* eapply inline_p_ps.
+  apply H.
+* eapply inline_p_ps.
+  apply H.
+* eapply inline_p_ps.
+  apply H.
+* inversion H;subst.
+  apply E_Seq with s'0.
+  + apply IHp1.
+    apply H2.
+  + apply IHp2.
+    apply H6.
+* inversion H;subst.
+  + apply E_IfTrue.
+    - assumption.
+    - apply IHp1.
+      assumption.
+  + apply E_IfFalse.
+    - assumption.
+    - apply IHp2.
+      assumption.
+* remember (CWhile b p inv) as original_command eqn:Horig.
+  induction H.
+  + inversion Horig.
+  + inversion Horig.
+  + inversion Horig.
+  + inversion Horig.
+  + inversion Horig.
+  + inversion Horig.
+  + inversion Horig;subst.
+     eapply E_WhileFalse.
+     assumption.
+  + inversion Horig;subst.
+    eapply E_WhileTrue.
+    - assumption.
+    - apply IHp. apply H0.
+    - apply IHceval2.
+      assumption.
+      reflexivity.
+  + inversion Horig;subst.
+* inversion H; subst.
+  rewrite inline_ccall.
+  eapply inline_p_ps.
+  apply H1.
+Qed.
+
+(* ceval is "n" inlining insensitive on command *)
+
+Lemma inline_n_ceval n p s ps_init s':
+  (forall ps, ceval (k_inliner n p ps_init) s ps s') -> ceval p s ps_init s'.
+Proof.
+intros.
+specialize (H ps_init).
+generalize dependent s.
+generalize dependent s'.
+generalize dependent p.
+generalize dependent ps_init.
+induction n.
+* intros.
+  apply ceval_inf_loop in H.
+  contradiction H.
+* induction p;intros.
+  + apply H.
+  + apply H.
+  + apply H.
+  + inversion H;subst.
+    apply E_Seq with s'0.
+    - apply IHp1.
+      apply H2.
+    - apply IHp2.
+      apply H6.
+  + inversion H;subst.
+    - apply E_IfTrue.
+      ** assumption.
+      ** apply IHp1.
+         assumption.
+    - apply E_IfFalse.
+      ** assumption.
+      ** apply IHp2.
+         assumption.
+   + remember (k_inliner (S n) (CWhile b p inv) ps_init) as original_command eqn:Horig.
+     induction H.
+     - inversion Horig.
+     - inversion Horig.
+     - inversion Horig.
+     - inversion Horig.
+     - inversion Horig.
+     - inversion Horig.
+     - inversion Horig;subst.
+       eapply E_WhileFalse.
+       assumption.
+     - inversion Horig;subst.
+       eapply E_WhileTrue.
+       ** assumption.
+       ** apply IHp. apply H0.
+       ** apply IHceval2.
+          assumption.
+          reflexivity.
+     - inversion Horig;subst.
+  + apply inline_ceval.
+    apply IHn.
+    rewrite inline_ccall in H.
+    apply H.
+Qed.
+
+Lemma inline_ceval_S n p s ps_init  s' ps:
+  ceval (k_inliner n p ps_init) s ps s' ->
+  forall m, n <= m -> ceval (k_inliner m p ps_init) s ps s'.
+Proof.
+intros.
+generalize dependent s.
+generalize dependent s'.
+generalize dependent p.
+generalize dependent m.
+induction n.
+* intros.
+  apply ceval_inf_loop in H.
+  contradiction H.
+* destruct m as [| m].
+  + intros. inversion H0.
+  + induction p;intros.
+    - apply H.
+    - apply H.
+    - apply H.
+    - rewrite inline_cseq in H.
+      inversion H;subst.
+      rewrite inline_cseq.
+      apply E_Seq with s'0.
+      ** apply IHp1.
+         apply H3.
+      ** apply IHp2.
+         apply H7.
+    - rewrite inline_cif in H.
+      inversion H;subst.
+      ** rewrite inline_cif.
+         apply E_IfTrue.
+         ++ assumption.
+         ++ apply IHp1.
+            apply H8.
+      ** rewrite inline_cif.
+         apply E_IfFalse.
+         ++ assumption.
+         ++ apply IHp2.
+            apply H8.
+     - remember (k_inliner (S n) (CWhile b p inv) ps_init) as original_command eqn:Horig.
+     induction H.
+      ** inversion Horig.
+      ** inversion Horig.
+      ** inversion Horig.
+      ** inversion Horig.
+      ** inversion Horig.
+      ** inversion Horig.
+      ** inversion Horig;subst.
+         eapply E_WhileFalse.
+         assumption.
+      ** inversion Horig;subst.
+         rewrite inline_cwhile.
+         eapply E_WhileTrue.
+         ++ assumption.
+         ++ apply IHp. apply H1.
+         ++ apply IHceval2.
+            assumption.
+            assumption.
+            reflexivity.
+      ** inversion Horig;subst.
+  - rewrite inline_ccall.
+    apply IHn.
+    now apply Le.le_S_n.
+    apply H.
+Qed.
+
+Lemma ceval_inline_n p s ps_init s':
+  ceval p s ps_init s' -> exists n, forall ps, ceval (k_inliner n p ps_init) s ps s'.
+Proof.
+induction 1;intros.
+* exists 1.
+  apply E_Skip.
+* exists 1.
+  intros.
+  apply E_Ass.
+  assumption.
+* exists 1.
+  intros.
+  apply E_Assert.
+  assumption.
+* destruct IHceval as [n IH].
+  exists n.
+  intros.
+  specialize (IH ps0).
+  destruct n.
+  - apply ceval_inf_loop in IH.
+    contradiction IH.
+  - rewrite inline_cif.
+    apply E_IfTrue.
+    assumption.
+    apply IH.
+* destruct IHceval as [n IH].
+  exists n.
+  intros.
+  specialize (IH ps0).
+  destruct n.
+  - apply ceval_inf_loop in IH.
+    contradiction IH.
+  - rewrite inline_cif.
+    apply E_IfFalse.
+    assumption.
+    apply IH.
+* destruct IHceval1 as [n1 IH1].
+  destruct IHceval2 as [n2 IH2].
+  exists (max n1 n2).
+  intros.
+  specialize (IH1 ps0).
+  specialize (IH2 ps0).
+  destruct n1 as [|n1].
+  + apply ceval_inf_loop in IH1.
+    contradiction IH1.
+  + destruct n2 as [|n2].
+    - apply ceval_inf_loop in IH2.
+      contradiction IH2.
+    - destruct (Proc.max_dec (S n1) (S n2)).
+      ** rewrite e.
+         rewrite inline_cseq.
+         apply E_Seq with s'. 
+         ++ apply inline_ceval_S with (S n1); [now auto | reflexivity].
+         ++ apply inline_ceval_S with (S n2); [now auto | now apply PeanoNat.Nat.max_l_iff].
+      ** rewrite e.
+         rewrite inline_cseq.
+         apply E_Seq with s'. 
+         ++ apply inline_ceval_S with (S n1); [now auto | now apply PeanoNat.Nat.max_r_iff].
+         ++ apply inline_ceval_S with (S n2); [now auto | reflexivity].
+* exists 1. intros. rewrite inline_cwhile. apply E_WhileFalse; now auto.
+* destruct IHceval1 as [n1 IH1].
+  destruct IHceval2 as [n2 IH2].
+  exists (max n1 n2).
+  intros.
+  specialize (IH1 ps0).
+  specialize (IH2 ps0).
+  destruct n1 as [|n1].
+  + apply ceval_inf_loop in IH1.
+    contradiction IH1.
+  + destruct n2 as [|n2].
+    - apply ceval_inf_loop in IH2.
+      contradiction IH2.
+    - destruct (Proc.max_dec (S n1) (S n2)).
+      ** rewrite e.
+         rewrite inline_cwhile.
+         apply E_WhileTrue with s'; [now auto | | ].
+         ++ apply inline_ceval_S with (S n1); [now auto | reflexivity].
+         ++ rewrite <- inline_cwhile.
+            apply inline_ceval_S with (S n2); [now auto | now apply PeanoNat.Nat.max_l_iff].
+      ** rewrite e.
+         rewrite inline_cwhile.
+         apply E_WhileTrue with s';[now auto | | ]. 
+         ++ apply inline_ceval_S with (S n1) ; [now auto | now apply PeanoNat.Nat.max_r_iff].
+         ++ rewrite <- inline_cwhile.
+            apply inline_ceval_S with (S n2); [now auto | reflexivity].
+* destruct IHceval as [n IH].
+  exists (S n).
+  intros.
+  specialize (IH ps0).
+  rewrite inline_ccall.
+  destruct n as [|n].
+  + apply ceval_inf_loop in IH.
+    contradiction IH.
+  + apply IH.
+Qed.
+
+(* ceval is inlining insensitive on ps *)
+
+Lemma n_inline_ps_ceval p s ps s' n:
+  ceval p s (k_inliner_ps n ps) s' -> ceval p s ps s'.
+Proof.
+intros.
+apply inline_n_ceval with (S n).
+intros.
+specialize (n_ps_inline_n_inline n p s ps s' H ps0).
+intros.
+apply H0.
+Qed.
+
+Lemma ceval_n_inline_ps p s ps s':
+  ceval p s ps s' -> exists n, ceval p s (k_inliner_ps n ps) s'.
+Proof.
+intros.
+apply ceval_inline_n in H.
+destruct H as [n IH].
+destruct n as [|n].
+* specialize (IH ps).
+  apply ceval_inf_loop in IH.
+  contradiction IH.
+* exists n.
+  apply n_inline_n_inline_ps.
+  apply IH.
+Qed.
+
+(*Inling "n+1" times on Psi.psi is equivalent to inline p and "n" times Psi.psi*)
+
+Lemma n_inline_ps_inline  n  f s ps s' :
+ ceval (CCall f) s (k_inliner_ps (S n) ps) s' ->
+ ceval (inliner (CCall f) ps) s (k_inliner_ps n ps) s'.
+Proof.
+intros.
+apply inline_ceval.
+specialize (n_ps_inline_n_inline (S n) (CCall f) s ps s' H).
+intros.
+apply H0.
+Qed.
